Just took a look and add indentation

hoare_wp.fst
@@ -319,90 +319,113 @@ let proof_if_false_temp c p1 p2 h lhs =
 
 val proof_if_false : c : pred -> p1 : pred -> p2 : pred -> h : heap -> Tot (deduce( FImpl (pand (pif c p1 p2) (pnot c) h ) (p2 h) ))
 let proof_if_false c p1 p2 h = 
-  DImplIntro (FAnd (pif c p1 p2 h) (pnot c h)) (p2 h) (proof_if_false_temp c p1 p2 h)
+    DImplIntro (FAnd (pif c p1 p2 h) (pnot c h)) (p2 h) (proof_if_false_temp c p1 p2 h)
 
 val plouf : q : pred -> h : heap -> deduce (q h) -> Tot (deduce (q h))
 let plouf q h p = p
 
-val while1 : be : bexp -> c : com -> i : pred -> q : pred -> deduce (FForall (pimpl i (pif (bpred be) (wlp c i) q))) -> h : heap ->
-deduce (pand i (bpred be) h) -> Tot (deduce (wlp c i h))
+val while1 : be : bexp -> c : com -> i : pred -> q : pred -> 
+            deduce (FForall (pimpl i (pif (bpred be) (wlp c i) q))) -> 
+            h : heap ->
+            deduce (pand i (bpred be) h) -> 
+            Tot (deduce (wlp c i h))
 let while1 be c i q vprop h vand =
-(* i h ==> if .... h *)
-  let v1 = DForallElim (pimpl i (pif (bpred be) (wlp c i) q )) vprop h in
-  let vih = DAndElim1 (i h) (bpred be h) vand in
-  let vbh = DAndElim2 (i h) (bpred be h) vand in
-  let v2 = DImplElim (i h) ((pif (bpred be) (wlp c i) q) h) v1 vih in
-  let v3 = DAndElim1 (pimpl (bpred be) (wlp c i) h) (pimpl (pnot (bpred be)) q h) v2 in
-  DImplElim (bpred be h) (wlp c i h) v3 vbh 
-val while2 : be : bexp -> c : com -> i : pred -> q : pred -> deduce (FForall (pimpl i (pif (bpred be) (wlp c i) q))) -> h : heap ->
-Tot (deduce (pimpl (pand i (bpred be)) (wlp c i) h))
+    (* i h ==> if .... h *)
+    let v1 = DForallElim (pimpl i (pif (bpred be) (wlp c i) q )) vprop h in
+    let vih = DAndElim1 (i h) (bpred be h) vand in
+    let vbh = DAndElim2 (i h) (bpred be h) vand in
+    let v2 = DImplElim (i h) ((pif (bpred be) (wlp c i) q) h) v1 vih in
+    let v3 = DAndElim1 (pimpl (bpred be) (wlp c i) h) (pimpl (pnot (bpred be)) q h) v2 in
+    DImplElim (bpred be h) (wlp c i h) v3 vbh 
+
+val while2 : be : bexp -> c : com -> i : pred -> q : pred -> 
+    deduce (FForall (pimpl i (pif (bpred be) (wlp c i) q))) -> 
+    h : heap ->
+    Tot (deduce (pimpl (pand i (bpred be)) (wlp c i) h))
 let while2 be c i q vprop h =
-DImplIntro (pand i (bpred be) h ) (wlp c i h) (while1 be c i q vprop h)
+    DImplIntro (pand i (bpred be) h ) (wlp c i h) (while1 be c i q vprop h)
 
-val while3 : be : bexp -> c : com -> i : pred -> q : pred -> deduce (FForall (pimpl i (pif (bpred be) (wlp c i) q))) -> h : heap ->
-deduce (wlp (While be c i) q h) -> Tot (deduce (i h))
+val while3 : be : bexp -> c : com -> i : pred -> q : pred -> 
+    deduce (FForall (pimpl i (pif (bpred be) (wlp c i) q))) -> 
+    h : heap ->
+    deduce (wlp (While be c i) q h) -> 
+    Tot (deduce (i h))
 let while3 be c i q vprop h vwlpcih =
-DAndElim1 (i h) (FForall (pimpl i (pif (bpred be) (wlp c i) q))) vwlpcih
-val while4 : be : bexp -> c : com -> i : pred -> q : pred -> deduce (FForall (pimpl i (pif (bpred be) (wlp c i) q))) -> h : heap ->
-Tot (deduce (pimpl (wlp (While be c i) q) i h))
+    DAndElim1 (i h) (FForall (pimpl i (pif (bpred be) (wlp c i) q))) vwlpcih
+
+val while4 : be : bexp -> c : com -> i : pred -> q : pred -> 
+    deduce (FForall (pimpl i (pif (bpred be) (wlp c i) q))) -> 
+    h : heap ->
+    Tot (deduce (pimpl (wlp (While be c i) q) i h))
 let while4 be c i q vprop h =
-DImplIntro (wlp (While be c i) q h) (i h) (while3 be c i q vprop h)
+    DImplIntro (wlp (While be c i) q h) (i h) (while3 be c i q vprop h)
 
-val while5 : be : bexp -> c : com -> i : pred -> q : pred -> deduce (FForall (pimpl i (pif (bpred be) (wlp c i) q))) -> h : heap ->
-deduce (pand i (pnot (bpred be)) h) -> Tot (deduce (q h))
+val while5 : be : bexp -> c : com -> i : pred -> q : pred -> 
+    deduce (FForall (pimpl i (pif (bpred be) (wlp c i) q))) -> 
+    h : heap ->
+    deduce (pand i (pnot (bpred be)) h) -> 
+    Tot (deduce (q h))
 let while5 be c i q vprop h vand =
-(* i h ==> if .... h *)
-  let v1 = DForallElim (pimpl i (pif (bpred be) (wlp c i) q )) vprop h in
-  let vih = DAndElim1 (i h) (pnot (bpred be) h) vand in
-  let vbnh = DAndElim2 (i h) (pnot (bpred be) h) vand in
-  let v2 = DImplElim (i h) ((pif (bpred be) (wlp c i) q) h) v1 vih in
-  let v3 = DAndElim2 (pimpl (bpred be) (wlp c i) h) (pimpl (pnot (bpred be)) q h) v2 in
-  DImplElim (pnot (bpred be) h) (q h) v3 vbnh 
-val while6 : be : bexp -> c : com -> i : pred -> q : pred -> deduce (FForall (pimpl i (pif (bpred be) (wlp c i) q))) -> h : heap ->
-Tot (deduce (pimpl (pand i (pnot (bpred be))) q h))
+    (* i h ==> if .... h *)
+    let v1 = DForallElim (pimpl i (pif (bpred be) (wlp c i) q )) vprop h in
+    let vih = DAndElim1 (i h) (pnot (bpred be) h) vand in
+    let vbnh = DAndElim2 (i h) (pnot (bpred be) h) vand in
+    let v2 = DImplElim (i h) ((pif (bpred be) (wlp c i) q) h) v1 vih in
+    let v3 = DAndElim2 (pimpl (bpred be) (wlp c i) h) (pimpl (pnot (bpred be)) q h) v2 in
+    DImplElim (pnot (bpred be) h) (q h) v3 vbnh 
+
+val while6 : be : bexp -> c : com -> i : pred -> q : pred -> 
+    deduce (FForall (pimpl i (pif (bpred be) (wlp c i) q))) -> 
+    h : heap ->
+    Tot (deduce (pimpl (pand i (pnot (bpred be))) q h))
 let while6 be c i q vprop h =
-DImplIntro (pand i (pnot (bpred be)) h ) (q h) (while5 be c i q vprop h)
+    DImplIntro (pand i (pnot (bpred be)) h ) (q h) (while5 be c i q vprop h)
 
 
-val whilecase : be : bexp -> c : com -> i : pred -> q : pred -> deduce (FForall (pimpl i (pif (bpred be) (wlp c i) q))) -> h : heap -> h' : heap -> hwlpi : hoare (wlp c i) c i -> Tot(hoare (wlp (While be c i) q) (While be c i) q)
+val whilecase : be : bexp -> c : com -> i : pred -> q : pred -> 
+    deduce (FForall (pimpl i (pif (bpred be) (wlp c i) q))) -> 
+    h : heap -> 
+    h' : heap -> 
+    hwlpi : hoare (wlp c i) c i -> 
+    Tot(hoare (wlp (While be c i) q) (While be c i) q)
 let whilecase be c i q vforall h h' hwlpi =
-(*forall. i /\ b ==> wlp c i *)
-let v1 = DForallIntro (pimpl (pand i (bpred be)) (wlp c i)) (while2 be c i q vforall) in
-(*forall. i ==> i*)
-let v2 = DForallIntro (pimpl i i) (fun h -> DImplIntro (i h) (i h) (plouf i h)) in
-(*{i /\ b} c i *)
-let  hibci = hoare_consequence (pand i (bpred be)) (wlp c i) i i c hwlpi v1 v2 in
-(*{i} While be c i {i /\ not be}*)
-let hiwhileinbe = hoare_while i be c hibci in
-(*forall. wlp c i ==> i*)
-let v3 = DForallIntro (pimpl (wlp (While be c i) q) i) (while4 be c i q vforall) in
-(*forall. i /\ not be ==> q*)
-let v4 = DForallIntro (pimpl (pand i (pnot (bpred be))) q) (while6 be c i q vforall) in
-hoare_consequence (wlp (While be c i) q) i q (pand i (pnot (bpred be))) (While be c i) hiwhileinbe v3 v4
+    (*forall. i /\ b ==> wlp c i *)
+    let v1 = DForallIntro (pimpl (pand i (bpred be)) (wlp c i)) (while2 be c i q vforall) in
+    (*forall. i ==> i*)
+    let v2 = DForallIntro (pimpl i i) (fun h -> DImplIntro (i h) (i h) (plouf i h)) in
+    (*{i /\ b} c i *)
+    let  hibci = hoare_consequence (pand i (bpred be)) (wlp c i) i i c hwlpi v1 v2 in
+    (*{i} While be c i {i /\ not be}*)
+    let hiwhileinbe = hoare_while i be c hibci in
+    (*forall. wlp c i ==> i*)
+    let v3 = DForallIntro (pimpl (wlp (While be c i) q) i) (while4 be c i q vforall) in
+    (*forall. i /\ not be ==> q*)
+    let v4 = DForallIntro (pimpl (pand i (pnot (bpred be))) q) (while6 be c i q vforall) in
+    hoare_consequence (wlp (While be c i) q) i q (pand i (pnot (bpred be))) (While be c i) hiwhileinbe v3 v4
 
 val wlp_sound : c:com -> q:pred -> Tot (hoare (wlp c q) c q)
 let rec wlp_sound c q =
   match c with
-  | Skip -> hoare_skip q
-  | Assign x e -> hoare_assign q x e
-  | Seq c1 c2 -> 
-      let wlp_c1 = wlp_sound c1 (wlp c2 q) in
-      let wlp_c2 = wlp_sound c2 q in
-      hoare_seq (wlp c1 (wlp c2 q)) c1 (wlp c2 q) c2 q wlp_c1 wlp_c2
-  | If be ct ce -> 
-      let wlp_t = wlp_sound ct q in
-      let wlp_e = wlp_sound ce q in
-      let vpp' = DForallIntro (pimpl (pand (pif (bpred be) (wlp ct q) (wlp ce q)) (bpred be)) (wlp ct q)) (proof_if_true (bpred be) (wlp ct q) (wlp ce q)) in 
-      let p = (pimpl (pand (pif (bpred be) (wlp ct q) (wlp ce q)) (bpred be)) (wlp ct q)) in
-      let p' = wlp ct q in
-      let hthen = hoare_consequence (pand (pif (bpred be) (wlp ct q) (wlp ce q)) (bpred be)) (wlp ct q) q q ct wlp_t vpp' (DForallIntro (pimpl q q) (fun (h:heap) -> (DImplIntro (q h) (q h) (plouf q h)))) in
-      let vpp'' = DForallIntro (pimpl (pand (pif (bpred be) (wlp ct q) (wlp ce q)) (pnot (bpred be))) (wlp ce q)) (proof_if_false (bpred be) (wlp ct q) (wlp ce q)) in 
-      let helse = hoare_consequence (pand (pif (bpred be) (wlp ct q) (wlp ce q)) (pnot (bpred be))) (wlp ce q) q q ce wlp_e vpp'' (DForallIntro (pimpl q q) (fun (h:heap) -> (DImplIntro (q h) (q h) (plouf q h)))) in
-      hoare_if (wlp c q) q be ct ce hthen helse
-  | While be body i -> (*Here we have to get the proof of the forall inside the argument, that is why we have to write this with lambda*)
-    fun h h' pr vph -> 
-    let vforall = DAndElim2 (i h) (FForall (pimpl i (pif (bpred be) (wlp body i) q))) vph in
-    whilecase be body i q vforall h h' (wlp_sound body i) pr vph
+    | Skip -> hoare_skip q
+    | Assign x e -> hoare_assign q x e
+    | Seq c1 c2 -> 
+        let wlp_c1 = wlp_sound c1 (wlp c2 q) in
+        let wlp_c2 = wlp_sound c2 q in
+        hoare_seq (wlp c1 (wlp c2 q)) c1 (wlp c2 q) c2 q wlp_c1 wlp_c2
+    | If be ct ce -> 
+        let wlp_t = wlp_sound ct q in
+        let wlp_e = wlp_sound ce q in
+        let vpp' = DForallIntro (pimpl (pand (pif (bpred be) (wlp ct q) (wlp ce q)) (bpred be)) (wlp ct q)) (proof_if_true (bpred be) (wlp ct q) (wlp ce q)) in 
+        let p = (pimpl (pand (pif (bpred be) (wlp ct q) (wlp ce q)) (bpred be)) (wlp ct q)) in
+        let p' = wlp ct q in
+        let hthen = hoare_consequence (pand (pif (bpred be) (wlp ct q) (wlp ce q)) (bpred be)) (wlp ct q) q q ct wlp_t vpp' (DForallIntro (pimpl q q) (fun (h:heap) -> (DImplIntro (q h) (q h) (plouf q h)))) in
+        let vpp'' = DForallIntro (pimpl (pand (pif (bpred be) (wlp ct q) (wlp ce q)) (pnot (bpred be))) (wlp ce q)) (proof_if_false (bpred be) (wlp ct q) (wlp ce q)) in 
+        let helse = hoare_consequence (pand (pif (bpred be) (wlp ct q) (wlp ce q)) (pnot (bpred be))) (wlp ce q) q q ce wlp_e vpp'' (DForallIntro (pimpl q q) (fun (h:heap) -> (DImplIntro (q h) (q h) (plouf q h)))) in
+        hoare_if (wlp c q) q be ct ce hthen helse
+    | While be body i -> (*Here we have to get the proof of the forall inside the argument, that is why we have to write this with lambda*)
+        fun h h' pr vph -> 
+            let vforall = DAndElim2 (i h) (FForall (pimpl i (pif (bpred be) (wlp body i) q))) vph in
+            whilecase be body i q vforall h h' (wlp_sound body i) pr vph
 
     
     
@@ -460,84 +483,128 @@ for now, I do not know how to change this definition in order to make it works �
 val skip : p : pred ->  q : pred -> hpcq : hoare p Skip q -> h : heap -> deduce (p h) -> Tot (deduce (q h))
 let skip p q hpcq h ph = hpcq (ESkip h) ph
 
-val assign1 : x : nat -> e : aexp -> p:pred -> q:pred -> hpcq : hoare_c p (Assign x e) q -> h : heap -> vph : deduce (p h) ->Tot( deduce(wlp (Assign x e) q h))
-
+val assign1 : x : nat -> e : aexp -> p:pred -> q:pred -> 
+          hpcq:hoare p (Assign x e) q -> 
+          h:heap -> 
+          vph:deduce (p h) ->
+          Tot( deduce(wlp (Assign x e) q h))
 let assign1  x e p q hpcq h vph =
-let h' = update h x (eval_aexp h e) in
-let pr = EAssign h x e in
-let vqh' = hpcq pr vph in
-vqh' 
+    let h' = update h x (eval_aexp h e) in
+    let pr = EAssign h x e in
+    let vqh' = hpcq pr vph in
+    vqh' 
 
-val assign2 : x : nat -> e : aexp -> p:pred -> q:pred -> hpcq : hoare_c p (Assign x e) q -> h : heap -> Tot(deduce (FImpl (p h) (wlp (Assign x e) q h)))
+val assign2 : x : nat -> e : aexp -> p:pred -> q:pred -> 
+          hpcq:hoare p (Assign x e) q -> 
+          h:heap -> 
+          Tot(deduce (FImpl (p h) (wlp (Assign x e) q h)))
 let assign2 x e p q hpcq h =
-DImplIntro (p h) (wlp (Assign x e) q h) (assign1 x e p q hpcq h)
+    DImplIntro (p h) (wlp (Assign x e) q h) (assign1 x e p q hpcq h)
 (*Idea of proof for the seq case, which do not typecheck.
 Anyway, there is a comparaison between two heaps, which
 is not computable …*)
 (*
-val seq1 : c1:com -> c2:com -> p : pred -> q:pred -> hpc1c2q :hoare_c p (Seq c1 c2) q -> h0 : heap -> vph0 : deduce (p h0) -> h1 : heap -> pr1 : reval c1 h0 h1 -> Tot(hoare_c (fun x -> FEq h1 x) c2 q)
+val seq1 : c1:com -> c2:com -> p : pred -> q:pred -> hpc1c2q :hoare p (Seq c1 c2) q -> h0 : heap -> vph0 : deduce (p h0) -> h1 : heap -> pr1 : reval c1 h0 h1 -> Tot(hoare (fun x -> FEq h1 x) c2 q)
 let seq1 c1 c2 p q hpc1c2q h0 vph0 h1 pr1 =  
-fun h1' h2 pr2 veq -> if h1 = h1' then hpc1c2q (ESeq pr1 pr2) vph0 
-else let vfalse = DImplElim (FEq h1 h1') FFalse (DNotEq h1 h1') veq in
-DFalseElim (q h2) vfalse
+    fun h1' h2 pr2 veq -> 
+        if h1 = h1' then 
+            hpc1c2q (ESeq pr1 pr2) vph0 
+        else 
+            let vfalse = DImplElim (FEq h1 h1') FFalse (DNotEq h1 h1') veq in
+            DFalseElim (q h2) vfalse
 *)
-val iftrue : be:bexp -> ct:com -> ce:com -> p : pred -> q:pred -> hpifq :hoare_c p (If be ct ce) q -> Tot(hoare_c (pand p (bpred be)) ct q)
-let iftrue be ct ce p q hpifq = fun h h' pr vpbeh ->
-if eval_bexp h be then
-hpifq (EIfTrue be ct ce pr) (DAndElim1 (p h) (bpred be h) vpbeh)
-else
-let vbe = DAndElim2 (p h) (bpred be h) vpbeh in
-let vnbe = DNotEq false true in
-let vfalse = DImplElim (bpred be h) FFalse vnbe vbe in
-DFalseElim (q h') vfalse
-val iffalse : be:bexp -> ct:com -> ce:com -> p : pred -> q:pred -> hpifq :hoare_c p (If be ct ce) q -> Tot(hoare_c (pand p (pnot (bpred be))) ce q)
-let iffalse be ct ce p q hpifq = fun h h' pr vpnbeh ->
-if eval_bexp h be = false then
-hpifq (EIfFalse be ct ce pr) (DAndElim1 (p h) (pnot (bpred be) h) vpnbeh)
-else
-let vnbe = DAndElim2 (p h) (pnot (bpred be) h) vpnbeh in
-let vbe = DEqRefl true in
-let vfalse = DImplElim (bpred be h) FFalse vnbe vbe in
-DFalseElim (q h') vfalse
+val iftrue : be:bexp -> ct:com -> ce:com -> p : pred -> q:pred -> 
+          hpifq:hoare p (If be ct ce) q -> 
+          Tot (hoare (pand p (bpred be)) ct q)
+let iftrue be ct ce p q hpifq = 
+    fun h h' pr vpbeh ->
+        if eval_bexp h be then
+            hpifq (EIfTrue be ct ce pr) (DAndElim1 (p h) (bpred be h) vpbeh)
+        else
+            let vbe = DAndElim2 (p h) (bpred be h) vpbeh in
+            let vnbe = DNotEq false true in
+            let vfalse = DImplElim (bpred be h) FFalse vnbe vbe in
+            DFalseElim (q h') vfalse
 
-val if5 : be :bexp -> ct : com -> ce:com -> p : pred -> q : pred -> vimpltrue : deduce(FForall(pimpl (pand p (bpred be)) (wlp ct q))) -> vimplfalse : deduce(FForall(pimpl (pand p (pnot (bpred be))) (wlp ce q))) -> h : heap -> vph : deduce(p h) -> vnbe : deduce (pnot (bpred be) h) -> Tot(deduce(wlp ce q h))
+val iffalse : be:bexp -> ct:com -> ce:com -> p : pred -> q:pred -> 
+          hpifq:hoare p (If be ct ce) q -> 
+          Tot (hoare (pand p (pnot (bpred be))) ce q)
+let iffalse be ct ce p q hpifq = 
+    fun h h' pr vpnbeh ->
+        if eval_bexp h be = false then
+            hpifq (EIfFalse be ct ce pr) (DAndElim1 (p h) (pnot (bpred be) h) vpnbeh)
+        else
+            let vnbe = DAndElim2 (p h) (pnot (bpred be) h) vpnbeh in
+            let vbe = DEqRefl true in
+            let vfalse = DImplElim (bpred be h) FFalse vnbe vbe in
+            DFalseElim (q h') vfalse
+
+val if5 : be :bexp -> ct : com -> ce:com -> p : pred -> q : pred -> 
+          vimpltrue:deduce(FForall(pimpl (pand p (bpred be)) (wlp ct q))) -> 
+          vimplfalse:deduce(FForall(pimpl (pand p (pnot (bpred be))) (wlp ce q))) -> 
+          h:heap -> 
+          vph:deduce(p h) -> 
+          vnbe:deduce (pnot (bpred be) h) -> 
+          Tot(deduce(wlp ce q h))
 let if5 be ct ce p q vimpltrue vimplfalse h vph vnbe =
-let vimplfalseh = DForallElim (pimpl (pand p (pnot (bpred be))) (wlp ce q)) vimplfalse h in
-let vand = DAndIntro (p h) (pnot (bpred be) h) vph vnbe in
-DImplElim (pand p (pnot (bpred be)) h) (wlp ce q h) vimplfalseh vand
+    let vimplfalseh = DForallElim (pimpl (pand p (pnot (bpred be))) (wlp ce q)) vimplfalse h in
+    let vand = DAndIntro (p h) (pnot (bpred be) h) vph vnbe in
+    DImplElim (pand p (pnot (bpred be)) h) (wlp ce q h) vimplfalseh vand
 
-val if4 : be :bexp -> ct : com -> ce:com -> p : pred -> q : pred -> vimpltrue : deduce(FForall(pimpl (pand p (bpred be)) (wlp ct q))) -> vimplfalse : deduce(FForall(pimpl (pand p (pnot (bpred be))) (wlp ce q))) -> h : heap -> vph : deduce(p h) -> vbe : deduce (bpred be h) -> Tot(deduce((wlp ct q) h))
+val if4 : be :bexp -> ct : com -> ce:com -> p : pred -> q : pred -> 
+          vimpltrue:deduce(FForall(pimpl (pand p (bpred be)) (wlp ct q))) -> 
+          vimplfalse:deduce(FForall(pimpl (pand p (pnot (bpred be))) (wlp ce q))) -> 
+          h:heap -> 
+          vph:deduce(p h) -> 
+          vbe:deduce (bpred be h) ->
+          Tot (deduce((wlp ct q) h))
 let if4 be ct ce p q vimpltrue vimplfalse h vph vbe =
-let vimpltrueh = DForallElim (pimpl (pand p (bpred be)) (wlp ct q)) vimpltrue h in
-let vand = DAndIntro (p h) (bpred be h) vph vbe in
-DImplElim (pand p (bpred be) h) (wlp ct q h) vimpltrueh vand
+    let vimpltrueh = DForallElim (pimpl (pand p (bpred be)) (wlp ct q)) vimpltrue h in
+    let vand = DAndIntro (p h) (bpred be h) vph vbe in
+    DImplElim (pand p (bpred be) h) (wlp ct q h) vimpltrueh vand
 
-val if3 : be :bexp -> ct : com -> ce:com -> p : pred -> q : pred -> vimpltrue : deduce(FForall(pimpl (pand p (bpred be)) (wlp ct q))) -> vimplfalse : deduce(FForall(pimpl (pand p (pnot (bpred be))) (wlp ce q))) -> h : heap -> vph : deduce(p h) -> Tot(deduce((pif (bpred be) (wlp ct q) (wlp ce q)) h))
+val if3 : be :bexp -> ct : com -> ce:com -> p : pred -> q : pred -> 
+          vimpltrue : deduce(FForall(pimpl (pand p (bpred be)) (wlp ct q))) -> 
+          vimplfalse : deduce(FForall(pimpl (pand p (pnot (bpred be))) (wlp ce q))) -> 
+          h : heap -> 
+          vph : deduce(p h) -> 
+          Tot (deduce((pif (bpred be) (wlp ct q) (wlp ce q)) h))
 let if3 be ct ce p q vimpltrue vimplfalse h vph =
-DAndIntro (pimpl (bpred be) (wlp ct q) h ) (pimpl (pnot (bpred be)) (wlp ce q) h) (DImplIntro (bpred be h) (wlp ct q h) (if4 be ct ce p q vimpltrue vimplfalse h vph)) (DImplIntro (pnot (bpred be) h) (wlp ce q h) (if5 be ct ce p q vimpltrue vimplfalse h vph))
+    DAndIntro (pimpl (bpred be) (wlp ct q) h ) (pimpl (pnot (bpred be)) (wlp ce q) h) (DImplIntro (bpred be h) (wlp ct q h) (if4 be ct ce p q vimpltrue vimplfalse h vph)) (DImplIntro (pnot (bpred be) h) (wlp ce q h) (if5 be ct ce p q vimpltrue vimplfalse h vph))
 
-val if2 : be :bexp -> ct : com -> ce:com -> p : pred -> q : pred -> vimpltrue : deduce(FForall(pimpl (pand p (bpred be)) (wlp ct q))) -> vimplfalse : deduce(FForall(pimpl (pand p (pnot (bpred be))) (wlp ce q))) -> h : heap -> Tot(deduce((pimpl p (pif (bpred be) (wlp ct q) (wlp ce q))) h))
+val if2 : be :bexp -> ct : com -> ce:com -> p : pred -> q : pred -> 
+          vimpltrue : deduce(FForall(pimpl (pand p (bpred be)) (wlp ct q))) -> 
+          vimplfalse : deduce(FForall(pimpl (pand p (pnot (bpred be))) (wlp ce q))) -> 
+          h : heap -> 
+          Tot(deduce((pimpl p (pif (bpred be) (wlp ct q) (wlp ce q))) h))
 let if2 be ct ce p q vimpltrue vimplfalse h =
-DImplIntro (p h) (pif (bpred be) (wlp ct q) (wlp ce q) h) (if3 be ct ce p q vimpltrue vimplfalse h)
-val if1 : be :bexp -> ct : com -> ce:com -> p : pred -> q : pred -> vimpltrue : deduce(FForall(pimpl (pand p (bpred be)) (wlp ct q))) -> vimplfalse : deduce(FForall(pimpl (pand p (pnot (bpred be))) (wlp ce q))) -> Tot(deduce(FForall(pimpl p (pif (bpred be) (wlp ct q) (wlp ce q)))))
+    DImplIntro (p h) (pif (bpred be) (wlp ct q) (wlp ce q) h) (if3 be ct ce p q vimpltrue vimplfalse h)
+
+val if1 : be :bexp -> ct : com -> ce:com -> p : pred -> q : pred -> 
+          vimpltrue : deduce(FForall(pimpl (pand p (bpred be)) (wlp ct q))) -> 
+          vimplfalse : deduce(FForall(pimpl (pand p (pnot (bpred be))) (wlp ce q))) -> 
+          Tot (deduce(FForall(pimpl p (pif (bpred be) (wlp ct q) (wlp ce q)))))
 let if1 be ct ce p q vimpltrue vimplfalse =
-DForallIntro (pimpl p (pif (bpred be) (wlp ct q) (wlp ce q))) (if2 be ct ce p q vimpltrue vimplfalse)
+    DForallIntro (pimpl p (pif (bpred be) (wlp ct q) (wlp ce q))) (if2 be ct ce p q vimpltrue vimplfalse)
 
 
 val wlp_weakest : c:com -> p:pred -> q:pred ->
             hpcq:hoare p c q -> 
             deduce (pred_impl p (wlp c q))
-
-let rec wlp_weakest c p q hpcq = match c with
-| Skip -> DForallIntro (pimpl p (wlp Skip q)) (fun h -> DImplIntro (p h) (wlp Skip q h) (skip p q hpcq h))
-| Assign x e -> DForallIntro (pimpl p (wlp (Assign x e) q)) (assign2 x e p q hpcq)
-(*The rule for Seq should be true. But my idea to 
-prove it can not be written in FStar … *)
-| Seq c1 c2 -> magic ()
-| If be ct ce -> let hoaretrue = iftrue be ct ce p q hpcq in
-let vimpltrue = wlp_weakest ct (pand p (bpred be)) q hoaretrue in
-let hoarefalse = iffalse be ct ce p q hpcq in
-let vimplfalse = wlp_weakest ce (pand p (pnot (bpred be))) q hoarefalse in
-if1 be ct ce p q vimpltrue vimplfalse
-(*It is anyway false for While*)
-| While be body i -> magic ()
+let rec wlp_weakest c p q hpcq = 
+    match c with
+      | Skip -> 
+          DForallIntro (pimpl p (wlp Skip q)) (fun h -> DImplIntro (p h) (wlp Skip q h) (skip p q hpcq h))
+      | Assign x e -> 
+          DForallIntro (pimpl p (wlp (Assign x e) q)) (assign2 x e p q hpcq)
+      (*The rule for Seq should be true. But my idea to 
+      prove it can not be written in FStar … *)
+      | Seq c1 c2 -> magic ()
+      | If be ct ce -> 
+          let hoaretrue = iftrue be ct ce p q hpcq in
+          let vimpltrue = wlp_weakest ct (pand p (bpred be)) q hoaretrue in
+          let hoarefalse = iffalse be ct ce p q hpcq in
+          let vimplfalse = wlp_weakest ce (pand p (pnot (bpred be))) q hoarefalse in
+          if1 be ct ce p q vimpltrue vimplfalse
+      (*It is anyway false for While*)
+      | While be body i -> magic ()
